\section{Example}\label{sec:example}

Let's take a domain language $E=<\Pi,\preceq,\Delta,\Phi>$ with :
\begin{itemize}
  \item $\Pi$ composed of 5 timepoints $t_0$ to $t_4$
  \item $\Delta$ only composed of the action $switch$
  \item $\Phi$ only composed of the fluent $light$
\end{itemize}

Let's take a domain description $D=<\gamma,\eta,\tau>$ with :
\begin{itemize}
  \item $\gamma$ composed of two c-proposition :
  \begin{itemize}
    \item $switch$ initiates $light$ when $\neg light$.
    \item $switch$ terminates $light$ when $light$.
  \end{itemize}
  \item $\eta$ composed of two h-proposition :
  \begin{itemize}
    \item $switch$ happens-at $t_1$.
    \item $switch$ happens-at $t_3$.
  \end{itemize}
  \item $\tau$ composed of no t-proposition.
\end{itemize}

Once translated we get :
\begin{itemize}
  %\item The length of the trace $length(\pi)=5$.
  \item The set of propositions $A$ composed of $switch$, $light$, $initiation(light)$ and $termination(light)$.
  \item The set of formulas $F$ composed of:
  \begin{itemize}
    \item The formulas taken from the propositions:
    \item $\alwaysF((switch\bigwedge \neg light)\rightarrow initiation(light))$
%    \item $\alwaysF(initiation(light)\rightarrow (switch\bigwedge \neg light))$
    \item $\alwaysF((switch\bigwedge light)\rightarrow termination(light))$
%    \item $\alwaysF(termination(light)\rightarrow (switch\bigwedge light))$
    \item $\next^{1}switch$
    \item $\next^{3}switch$
    \item $\next^{0}\neg switch$
    \item $\next^{2}\neg switch$
    \item $\next^{4}\neg switch$
    \item The formulas taken from the inertia axioms:
    \item $\alwaysF(light\rightarrow (termination(light) \release light))$
    \item $\alwaysF(\neg light\rightarrow (initiation(light) \release \neg light))$
    \item $\alwaysF(initiation(light)\rightarrow\wnext light)$
    \item $\alwaysF(termination(light)\rightarrow\wnext \neg light)$
  \end{itemize}
\end{itemize}

We can see that the original domain description had two models:
\begin{itemize}
  \item $H(light,t_0)=H(light,t_1)=H(light,t_4)=true$ and $H(light,t_2)=H(light,t_3)=false$
  \item $H(light,t_0)=H(light,t_1)=H(light,t_4)=false$ and $H(light,t_2)=H(light,t_3)=true$
\end{itemize}

Likewise, the resulting set of formulas only has two traces that respect them:
\begin{itemize}
  \item $\{light\}\{light,switch,termination(light)\}\{\}\{switch,initiation(light)\}(\{light\})^*$
  \item $\{\}\{switch,initiation(light)\}\{light\}\{light,switch,termination(light)\}(\{\})^*$
\end{itemize}
